#+TITLE: Pattern Recognition Homework 1

* 1:
** الف:
\begin{equation}
\[ \int_{-\infty}^{+\infty} (x + y)f(x,y)dxdy =  \int_{-\infty}^{+\infty} xf(x,y)dxdy + \int_{-\infty}^{+\infty} yf(x,y)dxdy \]
\[ =  \int_{-\infty}^{+\infty} xf_{X}(x,y)dx  + \int_{-\infty}^{ +\infty} yf_{Y}(x,y)dy = E[X]+E[Y] \]
\end{equation}

** ب:
\begin{equation}
\[\sigma^{2} = E[(X-\mu_{x})^{2}]  = E[X^{2} -2X\mu_{x} + \mu_{x}^{2}] = \]
\[ E[X^{2}] - 2E[X]\mu + E[\mu^{2}] = E[X^2] - 2\mu^2 + \mu^{2} = E[X^2] - \mu^{2} \]
\end{equation}

** پ:
Let X,Y be two independent random variable, that implies E[XY] = E[X]E[Y]. \\
now Cov(X,Y) = E[XY]-E[X]E[Y] = E[X]E[Y] - E[X]E[Y] = 0 \implies X,Y are Uncorrelated.

** ت:
Let X be a random variable with an estimated value greater than zero. \\
Let Y be a random variable independent of X with a zero estimated value. \\
Let Z be a random variable as Z = XY, therefore Z is dependent on both X and Y.\\
E[Z] = E[XY] = E[X]E[Y] = E[X] 0 = 0 \\
Cov (Z, X) = E[ZX] - E[Z]E[X] = 0 -  0.E[X] = 0 \implies X,Z are Uncorrelated.

** ث:
\begin{equation}
\[{X, Y are uncorolated \implies E[XY] = E[X]E[Y]}\]
\[\sigma^{2} = E[(X+Y)^{2}] - E[X+Y]^{2} = E[X^{2} + 2XY + Y^{2}] - (E[X]+E[Y])^{2} = \]
\[E[X^{2}] +2E[XY] + E[Y^{2} - E[X]^{2} -E[Y]^{2} - 2E[X]E[Y] \]
\[ = E[X^{2}] - E[X]^{2} + E[Y^{2}] -E[Y]^{2} +2E[XY]-2E[XY] = E[X^{2}] - E[X]^{2} + E[Y^{2}] -E[Y]^{2} = \sigma_{x} + \sigma_{y}\]
\end{equation}

** ج:
X_{1} and X_{2} are continuous random variables that implies P(X) for a single givin point is equal to zero.\\
\begin{equation}
P[X_{1} \leq X{2} ] = P[X_{1} < X_{2}] + P[x_{1} = X_{2}] = P[X_{1} < X_{2}] + 0 = P[X_{1} < X_{2}]
\end{equation}
X_{1} and X_{2} are independent and identically distributed So: \\
P[ X_{1} <  X_{2} ] =  P[X_{1} >  X{2} ]

\begin{equation}
\[\int_{\infty}^{+\infty} p(X) = 1 \implies 
2P{x_{1} \leq X_{2}] = 1 \implies
P[x_{1} \leq X_{2}] = \frac {1} {2}
\]
\end{equation}

** چ:

For Discrete random variable we can not assume  P(X) of any single point is equal to zero So we need P[X_{2}] and P[X_{1}].

* 2:
[]

* 3:

** p(y):
\begin{equation}
\[ p(y)=  \int_{-\infty}^{+\infty} p(x,y) dx = \int_{-\infty}^{+\infty} \frac{1}{2\pi a b} e^{-(\frac{(y-\mu)^{2})}{2a^{2}} + \frac{(x-y)^{2})}{2b^{2}})} dx = \]
\[ \int_{-\infty}^{+\infty} \frac{1}{2\pi a b} e^{-(\frac{(y-\mu)^{2}}{2a^{2}}}  e^{\frac{(x-y)^{2}}{2b^{2}})} dx = \]
\[  \frac{1}{\sqrt{2\pi a^{2}}} e^{-\frac{(y-\mu)^{2}}{2a^{2}}}  \int_{-\infty}^{+\infty}  \frac{1}{\sqrt{2\pi b^{2}}}  e^{- \frac{(x-y)^{2}}{2b^{2}}} dx = \]
\[  \frac{1}{\sqrt{2\pi a^{2}}} e^{-\frac{(y-\mu)^{2}}{2a^{2}}}  = \mathcal{N}(\mu,\,a^{2})\]
\end{equation}

** p(x):
\begin{equation}
\[ p(y)=  \int_{-\infty}^{+\infty} p(x,y) dy = \int_{-\infty}^{+\infty} \frac{1}{2\pi a b} e^{-(\frac{(y-\mu)^{2})}{2a^{2}} + \frac{(x-y)^{2})}{2b^{2}})} dy = \]
\[ \int_{-\infty}^{+\infty}  \frac{1}{2\pi a b} e^{ - (\frac{b^{2} (y-\mu)^2 + a^{2}(x-y)^2 } {2a^{2}b^{2}}) } dy = \]
\[ \int_{-\infty}^{+\infty} \frac{1}{2\pi a b} e^{-( \frac{ (a^{2}+b^{2})y^{2}-2(a^2x+b^2\mu)y+(b^2\mu^{2}+a^{2}x^{2}) }{2a^2b^2}  )} = \]
\[ \int_{-\infty}^{+\infty} \frac{1}{2\pi a b} e^{-( \frac{y^2-2\frac{a^2x+b^2\mu}{a^2+b^2}y+ \frac{b^2\mu^2+a^2x^2}{a^2+b^2}}{2\frac{a^2b^2}{a^2+b^2}} )} dy = \]
\[\int_{-\infty}^{+\infty} \frac{1}{2\pi a b} e^{-(\frac{y^2-2\frac{a^2x+b^2\mu}{a^2+b^2}y+\frac{b^2\mu^2+a^2x^2}{a^2+b^2}}{2\frac{a^2b^2}{a^2+b^2}})} dy = \]
\[\int_{-\infty}^{+\infty} \frac{1}{2\pi a b} e^{-(\frac{ y-\frac{a^2x+b^2\mu}{a^2+b^2}  }{2\frac{a^2b^2}{a^2+b^2}})} e^{-(\frac{  \frac{b^2\mu^2+a^2x^2}{a^2+b^2} - \frac{a^2x+b^2\mu}{a^2+b^2} }{2\frac{a^2b^2}{a^2+b^2}}) dy = \]
\[ \frac{1}{1\pi ab} \sqrt{2\pi \frac{a^2b^2}{a^2+b^2}} e^{-(\frac{  \frac{b^2\mu^2+a^2x^2}{a^2+b^2} - \frac{a^2x+b^2\mu}{a^2+b^2} }{2\frac{a^2b^2}{a^2+b^2}})} \int_{-\infty}^{+\infty} \frac{1}{2\pi a b} e^{-(\frac{ y-\frac{a^2x+b^2\mu}{a^2+b^2}  }{2\frac{a^2b^2}{a^2+b^2}})} dy =  \]
\[ \frac{1}{ \sqrt{2\pi (a^2+b^2)}} e^{-(\frac{  \frac{b^2\mu^2+a^2x^2}{a^2+b^2} - \frac{a^2x+b^2\mu}{a^2+b^2} }{2\frac{a^2b^2}{a^2+b^2}})} =  \]
\[ \frac{1}{ \sqrt{2\pi (a^2+b^2)}} e^{-( \frac{(x-\mu)^2}{2(a^2+b^2)}) } = \]
\[ \mathcal{N}(\mu,\,a^{2}+b^2)\]
\end{equation}

** p(x|y):
\begin{equation}
\[p(x|y) = \frac{p(x,y)}{p(y)} = \frac{ \frac{1}{2\pi a b} e^{-(\frac{(y-\mu)^{2})}{2a^{2}} + \frac{(x-y)^{2})}{2b^{2}})}   } { \frac{1} { \sqrt{2\pi a^2}} e^{ - \frac{(y-\mu)^2}{2a^2} }  } = \frac{1}{\sqrt{2 \pi b^2}} e^{- \frac{(x-y)^2}{ab^2}} =  \mathcal{N}(y, b^2)\]
\end{equation}

** p(y|x):
\begin{equation}
\[p(y|x) = \frac{p(x,y)}{p(y)} = \frac{ \frac{1}{2\pi a b} e^{-(\frac{(y-\mu)^{2})}{2a^{2}} + \frac{(x-y)^{2})}{2b^{2}})}   } { \frac{1}{ \sqrt{2\pi (a^2+b^2)}} e^{-( \frac{(x-\mu)^2}{2(a^2+b^2)}) } } = \frac{1}{ \sqrt{2 \pi \frac{a^2 b^2}{a^2 + b^2}} } e^{-( \frac{ ( y - \frac{a^2x+b^2\mu}{a^2+b^2})^2 }{ 2\frac{a^2b^2}{a^2+b^2} } )} = \mathcal{N}(\frac{a^2x+b^2\mu}{a^2+b^2},\,\frac{a^2b^2}{a^2+b^2})
\end{equation}
** Drawing:
Following octave code will produce graphics for this question.
#+begin_src octave
mu = 0;
a = 40;
b = 3;
x = 11.9

Y=[-50:0.1:50];

mean = ((a^2)*x+(b^2)*mu)/(a^2 + b^2);
var = ((a*b)^2)/(a^2+b^2);
Py_x = (1.0/sqrt(2*pi*var))*exp(-((Y-mean).^2)/(2*var));

var2 = a^2;
Py = (1.0 / sqrt(2*pi*var2))*exp(-((Y-mu).^2)/(2*var2));

plot(Y, Py_x, "b;p(y|x=11.9);");
hold on;
plot(Y,Py,'r;p(y);');


#+end_src
[[./graphs/hw1_3.jpg]]

* 4:
** الف:
A valid covariance matrix is symmetric and positive semi-definite.\\
\Sigma  = \Sigma^T Its symmetric.\\
\Sigma is positive semi-definite if all its eigenvalues are non-negative.[Next Part]\\
** ب:
\begin{equation}
\[\Sigma e = \lambda e \]
\[ (\Sigma -\lamdba I)e = 0 \]
\[ det (\Sigma - \lambda I) = 0  \implies (64 - \lambda)^2 - (-25)^2 = 0 \]
\[ 64^2 - 2 \times 64 \lambda + \lambda^2 + 25^2 = 0 \] 
\[ \lambda^2 -128\lambda  + 3471 = 0 \]
\[ \lambda = {39, 89} \]
\end{equation}

\begin{equation}
\[ (\Sigma - 39 \lambda)e = \begin{bmatrix}64 - 39 &-25 \\  -25 &64 - 39\end{bmatrix} \begin{bmatrix}a \\ b \end{bmatrix} = \begin{bmatrix}25 && -25 \\ -25 && 25 \end{bmatrix} \begin{bmatrix}a \\ b \end{bmatrix} =  \begin{bmatrix}0 \\ 0 \end{bmatrix}\] 
\[ a = b \implies \begin{bmatrix}1 \\1 \end{bmatrix}\]

\[ (\Sigma - 89 \lambda)e = \begin{bmatrix}64 - 89 &-25 \\  -25 &64 - 89\end{bmatrix} \begin{bmatrix}a \\ b \end{bmatrix} = \begin{bmatrix}-25 && -25 \\ -25 && -25 \end{bmatrix} \begin{bmatrix}a \\ b \end{bmatrix} =  \begin{bmatrix}0 \\ 0 \end{bmatrix}\] 
\[ a = -b \implies \begin{bmatrix}1 \\-1 \end{bmatrix}\]
\end{equation}

** پ:
Octave code returned normalized eigenvector.
#+begin_src octave
S = [64, -25; -25, 64];
[a, b] = eig(S)
#+end_src

a =
\\
  -0.70711  -0.70711\\
  -0.70711   0.70711\\

b =

Diagonal Matrix
\\
   39    0\\
    0   89\\
** ت:
I couldn't find any data attached I built my own data in data.mat. 
#+begin_src octave
S = [64, -25; -25, 64];
load ('data');

[eigvec, eigval] = eig(S);

Projected_data = (eigvec* X')';

subplot(121)
scatter(X(:,1), X(:,2), 'filled')
title ('Loaded DATA');

subplot(122)
scatter(Projected_data(:,1), Projected_data(:,2), 'filled')

title ('Projected DAtA');

#+end_src

[[./graphs/hw1_4.jpg]]
* 5:
** الف:
P(Y) = P(X_{1}) P(X_{2})
#+begin_src octave
function a = p_x(n)
a = zeros(size(n));
a( n <= 1) =1;
a( n < 0) = 0;
endfunction

X = [-2:0.1:2];
[X1, X2] = meshgrid (X, X);
Y = p_x(X1).*p_x(X2);
mesh (X1, X2, Y);
xlabel ("p(X1)");
ylabel ("p(X2)");
zlabel ("p(Y)");

#+end_src

[[./graphs/hw1_5_1.jpg]]

** ب:

\begin{equation}
P(X_{1} | y } = \frac{P(X_{1})P(X_{2})}{P(X_1)} = P(X_{2})
\end{equation}

#+begin_src octave
function a = p_x(n)
a = zeros(size(n));
a( n <= 1) =1;
a( n < 0) = 0;
endfunction

X = [-2:0.1:2];
[X1, Y] = meshgrid (X, X);
P_X_Y = p_x(X1);
mesh (X1, Y, P_X_Y);
xlabel ("p(X1)");
ylabel ("p(Y)");
zlabel ("p(X1|Y)");
#+end_src

[[./graphs/hw1_5_2.jpg]]

** پ:
*** P(Y) = \mathcal{N}(\mu_{X_{1}} + \mu_{X_{2}}, \sigma_{X_{1}}^2+\sigma_{X_{2}}^2)
\begin{equation}
\[ X_{1} ~  \mathcal{N}(\mu_{X_{1}}, \sigma_{X_{1}}^2) \]
\[ X_{2} ~  \mathcal{N}(\mu_{X_{2}}, \sigma_{X_{2}}^2) \]
\[ Z ~ X +Y \]
\[ Z ~ \mathcal{N}(\mu_{X_{1}} + \mu_{X_{2}}, \sigma_{X_{1}}^2+\sigma_{X_{2}}^2) \]
\end{equation}
\\
*** Proof:
\begin{equation}

\[
f_Z(z) 
&= \int_{-\infty}^{+\infty} 
   \frac{1}{\sqrt{2\pi}\sigma_Y}
   \exp \left[-{(z-x-\mu_Y)^2 \over 2\sigma_Y^2}\right]
   \frac{1}{\sqrt{2\pi}\sigma_X}
   \exp \left[-{(x-\mu_X)^2 \over 2\sigma_X^2}\right]
   \, dx 
\]
\[
&= \int_{-\infty}^{+\infty}
   \frac{1}{\sqrt{2\pi}\sqrt{2\pi}\sigma_X\sigma_Y}
   \exp \left[-\frac{\sigma_X^2(z-x-\mu_Y)^2 + \sigma_Y^2(x-\mu_X)^2}{2\sigma_X^2\sigma_Y^2}\right]
   \, dx 
\]
\[
&= \int_{-\infty}^{+\infty}
   \frac{1}{\sqrt{2\pi}\sqrt{2\pi}\sigma_X\sigma_Y}
   \exp \left[
      -\frac
         {\sigma_X^2(z^2 + x^2 + \mu_Y^2 - 2xz - 2z\mu_Y + 2x\mu_Y) + \sigma_Y^2(x^2 + \mu_X^2 - 2x\mu_X)}
         {2\sigma_Y^2\sigma_X^2}
   \right]
   \, dx 
\]
\[
&= \int_{-\infty}^{+\infty}
   \frac{1}{\sqrt{2\pi}\sqrt{2\pi}\sigma_X\sigma_Y}
   \exp_\left[
      -\frac
         {
            x^2(\sigma_X^2 + \sigma_Y^2) - 
            2x(\sigma_X^2(z - \mu_Y) + \sigma_Y^2\mu_X) +
            \sigma_X^2(z^2 + \mu_Y^2 - 2z\mu_Y) + \sigma_Y^2\mu_X^2
         }
         {2\sigma_Y^2\sigma_X^2}
   \right]
   \, dx
\]


\[Defining\ \sigma_Z = \sqrt{\sigma_X^2 + \sigma_Y^2} \]

\[
f_Z(z)
&= \int_{-\infty}^\infty
   \frac{1}{\sqrt{2\pi}\sigma_Z}
   \frac{1}{\sqrt{2\pi}\frac{\sigma_X\sigma_Y}{\sigma_Z}}
   \exp \left[
      -\frac
         {
            x^2 - 
            2x\frac{\sigma_X^2(z - \mu_Y) + \sigma_Y^2\mu_X}{\sigma_Z^2} +
            \frac{\sigma_X^2(z^2 + \mu_Y^2 - 2z\mu_Y) + \sigma_Y^2\mu_X^2}{\sigma_Z^2}
         }
         {2\left(\frac{\sigma_X\sigma_Y}{\sigma_Z}\right)^2}
   \right]
   \, dx 
\]

\[
&= \int_{-\infty}^\infty
   \frac{1}{\sqrt{2\pi}\sigma_Z}
   \frac{1}{\sqrt{2\pi}\frac{\sigma_X\sigma_Y}{\sigma_Z}}
   \exp \left[
      -\frac
         {
            \left(x - \frac{\sigma_X^2(z - \mu_Y) + \sigma_Y^2\mu_X}{\sigma_Z^2}\right)^2 -
            \left(\frac{\sigma_X^2(z - \mu_Y) + \sigma_Y^2\mu_X}{\sigma_Z^2}\right)^2 +
            \frac{\sigma_X^2(z - \mu_Y)^2 + \sigma_Y^2\mu_X^2}{\sigma_Z^2}
         }
         {2\left(\frac{\sigma_X\sigma_Y}{\sigma_Z}\right)^2}
   \right]
   \, dx 
\]

\[

&= \int_{-\infty}^\infty
   \frac{1}{\sqrt{2\pi}\sigma_Z}
   \exp _\left[
      -\frac
         {
            \sigma_Z^2\left(\sigma_X^2(z - \mu_Y)^2 + \sigma_Y^2\mu_X^2\right) -
            \left(\sigma_X^2(z - \mu_Y) + \sigma_Y^2\mu_X\right)^2
         }
         {2\sigma_Z^2\left(\sigma_X\sigma_Y\right)^2}
   \right]
   \frac{1}{\sqrt{2\pi}\frac{\sigma_X\sigma_Y}{\sigma_Z}}
   \exp _\left[
      -\frac
         {
            \left(x - \frac{\sigma_X^2(z - \mu_Y) + \sigma_Y^2\mu_X}{\sigma_Z^2}\right)^2
         }
         {2\left(\frac{\sigma_X\sigma_Y}{\sigma_Z}\right)^2}
   \right]
   \, dx 
\]
\[
&= \frac{1}{\sqrt{2\pi}\sigma_Z}
   \exp \left[ - { (z-(\mu_X+\mu_Y))^2 \over 2\sigma_Z^2 } \right]
   \int_{-\infty}^{\infty}
   \frac{1}{\sqrt{2\pi}\frac{\sigma_X\sigma_Y}{\sigma_Z}}
   \exp \left[ - \frac{\left(x-\frac{\sigma_X^2(z-\mu_Y)+\sigma_Y^2\mu_X}{\sigma_Z^2}\right)^2}{2\left(\frac{\sigma_X\sigma_Y}{\sigma_Z}\right)^2} \right]
   \, dx
\]
\[
f_Z(z) = \frac{1}{\sqrt{2\pi}\sigma_Z} \exp \left[ - { (z-(\mu_X+\mu_Y))^2 \over 2\sigma_Z^2 } \right]
\]
\end{equation}


*** Drawing:

#+begin_src octave
X = [-10:0.1:10];
plot (X, normpdf(X,0,2))
#+end_src

[[./graphs/hw1_5_3.jpg]]
